Logic/Predicate/FirstOrder/Arith/Hierarchy.lean
@@ -1,0 +1,55 @@
+import Logic.Predicate.FirstOrder.Eq
+
+variable {L : Language.{u}} [L.ORing] {μ : Type v}
+
+namespace SubTerm
+
+@[simp]
+def bZeroFree : SubTerm L μ (n + 1) → Bool
+  | #x       => x ≠ 0
+  | &_       => true
+  | func _ v => ∀ i, (v i).bZeroFree 
+
+lemma bShift_of_bZeroFree : ∀ {t : SubTerm L μ (n + 1)}, t.bZeroFree → ∃ u : SubTerm L μ n , t = u.bShift
+  | #x,       h => by
+    cases' x using Fin.cases with x
+    · simp at h
+    · exact ⟨#x, by simp⟩
+  | &x,       _ => ⟨&x, by simp⟩
+  | func f v, h => by
+    simp[bZeroFree] at h
+    choose w hw using fun i => bShift_of_bZeroFree (h i)
+    exact ⟨func f w, by simp[bShift_func]; funext; simp[hw]⟩
+
+end SubTerm
+
+namespace FirstOrder
+
+namespace Arith
+
+namespace Hierarchy
+
+inductive DeltaZero : ∀ {n}, SubFormula L μ n → Prop
+  | qfree {n} : ∀ {p : SubFormula L μ n}, p.qfree → DeltaZero p
+  | ballFvar {n} {p : SubFormula L μ (n + 1)} {x : Fin (n + 1)} (h : x ≠ 0) :
+    DeltaZero p → DeltaZero “∀[#0 < #x] !p”
+  | bexFvar {n} {p : SubFormula L μ (n + 1)} {x : Fin (n + 1)} (h : x ≠ 0) :
+    DeltaZero p → DeltaZero “∃[#0 < #x] !p”
+
+mutual
+
+inductive Sigma : ℕ → ∀ {n}, SubFormula L μ n → Prop
+  | zero {n} {p : SubFormula L μ n} : DeltaZero p → Sigma 0 p
+  | succ {n k} {p : SubFormula L μ (n + 1)} : Pi k p → Sigma (k + 1) (∃' p)
+
+inductive Pi : ℕ → ∀ {n}, SubFormula L μ n → Prop
+  | zero {n} {p : SubFormula L μ n} : DeltaZero p → Pi 0 p
+  | succ {n k} {p : SubFormula L μ (n + 1)} : Sigma k p → Pi (k + 1) (∀' p)
+
+end
+
+end Hierarchy
+
+end Arith
+
+end FirstOrder
