Logic/Predicate/FirstOrder/Arith/Theory.lean
@@ -1,0 +1,74 @@
+import Logic.Predicate.FirstOrder.Eq
+import Logic.Predicate.FirstOrder.Arith.Hierarchy
+
+namespace FirstOrder
+
+variable {L : Language.{u}} [L.ORing]
+
+namespace Arith
+
+def succInd (p : SubFormula L μ 1) : Formula L μ := “!p⟦0⟧ → ∀ (!p⟦#0⟧ → !p⟦#0 + 1⟧) → ∀ !p”
+
+def leastNumber (p : SubFormula L μ 1) : Formula L μ := “∃ !p → ∃ (!p ∧ ∀[#0 < #1] ¬!p⟦#0⟧)”
+
+def orderInd (p : SubFormula L μ 1) : Formula L μ := “∀ (∀[#0 < #1] !p⟦#0⟧ → !p⟦#0⟧) → ∀ !p”
+
+end Arith
+
+namespace Theory
+
+namespace Arith
+
+variable (L)
+
+inductive Robinson : Theory L
+  | q₁ : Robinson “∀ #0 + 1 ≠ 0”
+  | q₂ : Robinson “∀ ∀ (#0 + 1 = #1 + 1 → #0 = #1)”
+  | q₃ : Robinson “∀ (#0 = 0 ∨ (∃ #1 = #0 + 1))”
+  | q₄ : Robinson “∀ #0 + 0 = #0”
+  | q₅ : Robinson “∀ ∀ (#0 + (#1 + 1) = (#0 + #1) + 1)”
+  | q₆ : Robinson “∀ #0 * 0 = 0”
+  | q₇ : Robinson “∀ ∀ (#0 * (#1 + 1) = #0 * #1 + #0)”
+  | q₈ : Robinson “∀ ∀ (#0 < #1 ↔ (∃ #0 + #1 + 1 = #2))”
+
+inductive Ind (U : Set (SubSentence L 1)) : Theory L
+  | intro {σ} : σ ∈ U → Ind U (Arith.succInd σ) 
+
+section Paring
+variable [L.Pairing]
+
+inductive Pairing : Sentence L → Prop
+  | pairing : Pairing “∀ ∀ ∀ (⟨#0, #1⟩ = #2 ↔ (#0 + #1 + 1) * (#0 + #1) + 2 * #0 = 2 * #2)”
+
+end Paring
+
+section Exp
+variable [L.Exp]
+
+inductive Exp : Theory L
+  | zero : Exp “exp 0 = 1”
+  | succ : Exp “∀ exp (#0 + 1) = exp #0 * 2”
+
+end Exp
+
+end Arith
+
+class RobinsonTheory (T : Theory L) extends EqTheory T where
+  robinson : Arith.Robinson L ⊆ T
+
+class IndTheory (U) (T : Theory L) extends RobinsonTheory T where
+  ind : Arith.Ind L U ⊆ T
+
+abbrev IOpen (T : Theory L) := IndTheory SubFormula.qfree T
+
+abbrev ISigma (k : ℕ) (T : Theory L) := IndTheory (Arith.Hierarchy.Sigma k) T
+
+abbrev IPi (k : ℕ) (T : Theory L) := IndTheory (Arith.Hierarchy.Pi k) T
+
+abbrev Peano (T : Theory L) := IndTheory Set.univ T
+
+abbrev PairingTheory [L.Pairing] (T : Theory L) := SubTheory (Arith.Pairing L) T
+
+end Theory
+
+end FirstOrder
